Update tests to remove canonical value obligations

StrataTest/DL/Lambda/LExprEvalTests.lean
@@ -109,7 +109,6 @@ def test2 := TestCase.mk
 example: steps_well test2 := by
   unfold steps_well Scopes.toEnv test2
   take_step; apply Step.reduce_2 <;> try inhabited_metadata
-  · discharge_isCanonicalValue
   · repeat constructor
   take_step; reduce_beta
   take_step; constructor <;> try inhabited_metadata
@@ -345,11 +344,9 @@ example: steps_well test12 := by
   unfold steps_well Scopes.toEnv test12
   take_step; apply Step.reduce_1; inhabited_metadata; apply Step.reduce_2
   · inhabited_metadata;
-  · discharge_isCanonicalValue
   · reduce_beta
   take_step; apply Step.reduce_1; inhabited_metadata; apply Step.reduce_2;
   · inhabited_metadata;
-  · discharge_isCanonicalValue
   · apply Step.eval_fn <;> try discharge_isCanonicalValue
     · inhabited_metadata
   take_step; apply Step.reduce_1; inhabited_metadata; reduce_beta
@@ -427,38 +424,29 @@ example: stuck test15 := by
     cases a3
     cases a2; unfold denoteInt at he; contradiction
 
-
 def test16 := TestCase.mk
   testState
-  esM[((~Int.Add x) (~Int.Neg #30))]
-  esM[((~Int.Add x) #-30)]
+  esM[((λ %0) ((~Int.Add #20) #30))]
+  esM[(#50)]
 
 /-- info: true -/
 #guard_msgs in
 #eval check test16
 
--- test16 stucks because '~Int.Add x' isn't canonical value.
-example: stuck test16 := by
-  intros e H
-  cases H <;> try contradiction
-  case reduce_2 =>
-    rename_i a a2
-    conv at a => lhs; unfold isCanonicalValue; reduce; unfold isCanonicalValue; reduce
-    contradiction
-  case expand_fn =>
-    rename_i a a2 a3
-    cases a2
-    contradiction
-  case eval_fn =>
-    rename_i a a2 a3 he
-    cases a3
-    cases a2; unfold denoteInt at he; contradiction
+example: steps_well test16 := by
+  unfold steps_well Scopes.toEnv test16
+  take_step; apply Step.reduce_2
+  · inhabited_metadata
+  · apply Step.eval_fn <;> try discharge_isCanonicalValue
+    · inhabited_metadata
+  take_step; reduce_beta
+  take_refl
 
 
 def test17 := TestCase.mk
   testState
-  esM[((λ %0) ((~Int.Add #20) #30))]
-  esM[(#50)]
+  esM[((~Int.Div #300) ((~Int.Add #2) #1))]
+  esM[(#100)]
 
 /-- info: true -/
 #guard_msgs in
@@ -468,27 +456,6 @@ example: steps_well test17 := by
   unfold steps_well Scopes.toEnv test17
   take_step; apply Step.reduce_2
   · inhabited_metadata
-  · discharge_isCanonicalValue
-  · apply Step.eval_fn <;> try discharge_isCanonicalValue
-    · inhabited_metadata
-  take_step; reduce_beta
-  take_refl
-
-
-def test18 := TestCase.mk
-  testState
-  esM[((~Int.Div #300) ((~Int.Add #2) #1))]
-  esM[(#100)]
-
-/-- info: true -/
-#guard_msgs in
-#eval check test18
-
-example: steps_well test18 := by
-  unfold steps_well Scopes.toEnv test18
-  take_step; apply Step.reduce_2
-  · inhabited_metadata
-  · discharge_isCanonicalValue
   · apply Step.eval_fn <;> try discharge_isCanonicalValue
     · inhabited_metadata
   take_step; apply Step.eval_fn <;> try discharge_isCanonicalValue
@@ -497,21 +464,20 @@ example: steps_well test18 := by
   take_refl
 
 
-def test19 := TestCase.mk
+def test18 := TestCase.mk
   testState
   esM[((~Int.Add #3) (~Int.Neg #3))]
   esM[(#0)]
 
 /-- info: true -/
 #guard_msgs in
-#eval check test19
+#eval check test18
 
-example: steps_well test19 := by
-  unfold steps_well Scopes.toEnv test19
+example: steps_well test18 := by
+  unfold steps_well Scopes.toEnv test18
   take_step
   · apply Step.reduce_2
     · inhabited_metadata
-    · discharge_isCanonicalValue
     · apply Step.eval_fn <;> try discharge_isCanonicalValue
       · inhabited_metadata
   take_step
@@ -520,22 +486,21 @@ example: steps_well test19 := by
   take_refl
 
 
-def test20 := TestCase.mk
+def test19 := TestCase.mk
   testState
   esM[((~Int.Add (~Int.Neg #3)) #3)]
   esM[(#0)]
 
 /-- info: true -/
 #guard_msgs in
-#eval check test20
+#eval check test19
 
-example: steps_well test20 := by
-  unfold steps_well Scopes.toEnv test20
+example: steps_well test19 := by
+  unfold steps_well Scopes.toEnv test19
   take_step; apply Step.reduce_1
   · inhabited_metadata
   · apply Step.reduce_2
     · inhabited_metadata
-    · discharge_isCanonicalValue
     · apply Step.eval_fn <;> try discharge_isCanonicalValue
       · inhabited_metadata
   take_step; apply Step.eval_fn <;> try discharge_isCanonicalValue
@@ -543,37 +508,46 @@ example: steps_well test20 := by
   take_refl
 
 
-def test21 := TestCase.mk
+def test20 := TestCase.mk
   testState
   esM[((~Int.Div #300) ((~Int.Add #3) (~Int.Neg #3)))]
   esM[((~Int.Div #300) #0)]
 
 /-- info: true -/
 #guard_msgs in
-#eval check test21
+#eval check test20
 
-example: steps_well test21 := by
-  unfold steps_well Scopes.toEnv test21
+example: steps_well test20 := by
+  unfold steps_well Scopes.toEnv test20
   take_step; apply Step.reduce_2
   · inhabited_metadata
-  · discharge_isCanonicalValue
   · apply Step.reduce_2
     · inhabited_metadata
-    · discharge_isCanonicalValue
     · apply Step.eval_fn <;> try discharge_isCanonicalValue
       · inhabited_metadata
   take_step; apply Step.reduce_2
   · inhabited_metadata
-  · discharge_isCanonicalValue
   · apply Step.eval_fn <;> try discharge_isCanonicalValue
     · inhabited_metadata
   take_refl
 
 
-def test22 := TestCase.mk
+def test21 := TestCase.mk
   testState
   esM[((~Int.Div x) ((~Int.Add #2) #1))]
   esM[((~Int.Div x) #3)]
+
+/-- info: true -/
+#guard_msgs in
+#eval check test21
+
+-- TODO: steps_well proof of test21
+
+
+def test22 := TestCase.mk
+  testState
+  esM[((~Int.Le ((~Int.Div #300) ((~Int.Add #2) #1))) x)]
+  esM[((~Int.Le #100) x)]
 
 /-- info: true -/
 #guard_msgs in
@@ -584,38 +558,26 @@ def test22 := TestCase.mk
 
 def test23 := TestCase.mk
   testState
-  esM[((~Int.Le ((~Int.Div #300) ((~Int.Add #2) #1))) x)]
-  esM[((~Int.Le #100) x)]
+  esM[((~Int.Le ((~Int.Div #300) ((~Int.Add #2) y))) x)]
+  esM[((~Int.Le ((~Int.Div #300) ((~Int.Add #2) y))) x)]
 
 /-- info: true -/
 #guard_msgs in
 #eval check test23
 
--- TODO: steps_well proof of test23
+-- TODO: stuck proof of test23
 
 
 def test24 := TestCase.mk
-  testState
-  esM[((~Int.Le ((~Int.Div #300) ((~Int.Add #2) y))) x)]
-  esM[((~Int.Le ((~Int.Div #300) ((~Int.Add #2) y))) x)]
-
-/-- info: true -/
-#guard_msgs in
-#eval check test24
-
--- TODO: stuck proof of test24
-
-
-def test25 := TestCase.mk
   testState
   esM[((~Int.Div x) x)]
   esM[((~Int.Div x) x) ]
 
 /-- info: true -/
 #guard_msgs in
-#eval check test25
+#eval check test24
 
--- TODO: stuck proof of test25
+-- TODO: stuck proof of test24
 
 
 end EvalTest
